Inhabited OPreds. Still need to prove lemmas in core.v.

src/OPred.v
@@ -3,7 +3,7 @@
   ===========================================================================*)
 Require Import ssreflect ssrfun ssrbool eqtype fintype finfun seq tuple.
 Require Import bitsrep ioaction ilogic.
-Require Import Setoid CSetoid RelationClasses Morphisms.
+Require Import Setoid CSetoid RelationClasses Morphisms Program.Basics.
 
 Set Implicit Arguments.
 Unset Strict Implicit.
@@ -11,78 +11,115 @@ Import Prenex Implicits.
 
 Local Obligation Tactic := idtac.
 
-Definition OPred := ILFunFrm Actions Prop. 
-
-Local Existing Instance ILFun_Ops.
-Local Existing Instance ILFun_ILogic.
-
-Instance OLogicOps : ILogicOps OPred := _.
-Instance OLogic : ILogic OPred := _. 
-
-Implicit Arguments mkILFunFrm [[e] [ILOps]].
-
-Definition mkOPred (P : Actions -> Prop) 
-        (f : forall t t', t === t' -> P t |-- P t') : OPred := mkILFunFrm _ _ P f.
+(* We require predicates on observations to be non-empty i.e. for there to be
+   some sequence of actions for which it holds *)
+Record OPred := mkOPred {
+  OPred_pred :> Actions -> Prop;
+  OPred_inhabited: exists x: Actions, OPred_pred x
+}.
 
 Implicit Arguments mkOPred [].
 
+(* Singleton predicate *)
 Program Definition eq_opred s := mkOPred (fun s' => s === s') _.
-Next Obligation. move => s t t' EQ. by rewrite EQ. Qed.
+Next Obligation. move => s. by exists s. Qed. 
 
+(* The empty sequence of actions *)
+Definition empOP : OPred := eq_opred nil.
+
+(* A single output action *)
+Definition outOP (c:Chan) (d:Data) : OPred := eq_opred [::Out c d]. 
+
+(* A sequence of actions that splits into the concatenation of one
+satisfying P and one satisfying Q *)
 Program Definition catOP (P Q: OPred) : OPred
- := @mkILFunFrm _ _ Prop _ (fun o => exists o1 o2, o = o1++o2 /\ P o1 /\ Q o2) _.
+ := mkOPred (fun o => exists o1 o2, o = o1++o2 /\ P o1 /\ Q o2) _.
 Next Obligation.
-move => P Q o o' EQ [o1 [o2 [H1 [H2 H3]]]]. 
-exists o1, o2. by subst.
+move => [P [Px PH]] [Q [Qx QH]]. exists (Px++Qx). exists Px, Qx. 
+intuition. 
 Qed.
 
-Program Definition empOP : OPred :=   
-  mkILFunFrm _ _ (fun o => o = nil) _.
-Next Obligation.
-move => o o' EQ. by setoid_rewrite EQ. 
-Qed. 
+(* Any sequence of actions *)
+Program Definition trueOP : OPred := @mkOPred (fun _ => True) _. 
+Next Obligation. by exists nil. Qed. 
+
+(* Inclusion and equivalence on predicates *)
+Definition entailsOP (O O': OPred) := forall s, O s -> O' s. 
+Definition equivOP (O O': OPred) := entailsOP O O' /\ entailsOP O' O.
+
+Global Instance equivOPEquiv : Equiv OPred := equivOP.
+
+Global Instance entailsOPpre : PreOrder entailsOP.
+Proof. constructor; hnf. move => P s. intuition. 
+move => P Q R H1 H2 s. intuition. Qed. 
 
 
-Local Transparent ILFun_Ops ILPre_Ops.
+Global Instance equivOP_entailOP : subrelation equivOP entailsOP.
+Proof. firstorder. Qed.
 
-Instance catOP_entails_m: Proper (lentails ==> lentails ==> lentails) catOP.
+Global Instance equivOP_inverse_entailsOP: subrelation equivOP (inverse entailsOP).
+Proof. firstorder. Qed.
+
+Global Instance equivOP_entailsOP_m : Proper (equivOP ==> equivOP ==> iff) entailsOP.
+Proof. move => P P' HP Q Q' QP. split => H s H'; firstorder. Qed. 
+
+Global Instance entailsOP_entailsOP_m: Proper (entailsOP --> entailsOP ++> impl) entailsOP.
+Proof. move => P P' HP Q Q' QP H s H'. intuition. Qed.
+
+(* Morphisms for operators *)
+Instance catOP_entails_m: Proper (entailsOP ==> entailsOP ==> entailsOP) catOP.
 Proof.
 move => O1 O1' HO1 O2 O2' HO2. move => s/= H. 
 destruct H as [o1 [o2 [H1 [H2 H3]]]]. subst. 
 exists o1, o2. split => //. split. by apply HO1. by apply HO2. 
 Qed. 
 
-Instance catSP_lequiv_m: Proper (lequiv ==> lequiv ==> lequiv) catOP.
-Proof.
-  intros P P' HP Q Q' HQ.
-  split; apply catOP_entails_m; (apply HP || apply HQ).
-Qed.
+Instance catOP_equiv_m: Proper (equivOP ==> equivOP ==> equivOP) catOP.
+Proof. move => P P' HP Q Q' HQ. split; apply catOP_entails_m; (apply HP || apply HQ). Qed. 
 
-Definition outOP (c:Chan) (d:Data) : OPred := eq_opred [::Out c d]. 
-Definition seqOP (o:Actions) : OPred := eq_opred o.
-
-Lemma empOPR P : catOP P empOP -|- P.
-Proof.
-split.
-move => o [s1 [s2 [-> [H2 ->]]]]. by rewrite cats0. 
+(* catOP has empOP has left and right unit, and is associative *)
+Lemma empOPR P : equivOP (catOP P empOP) P.
+Proof. split.
+move => o [s1 [s2 [-> [H2 /= E2]]]]. by rewrite -E2 cats0. 
 move => o H. exists o, nil. by rewrite cats0. 
 Qed. 
 
-Lemma empOPL P : catOP empOP P -|- P.
-Proof.
-split.
-by move => o [s1 [s2 [-> [-> H]]]]. 
-move => o H. by exists nil, o. 
+Lemma empOPL P : equivOP (catOP empOP P) P.
+Proof. split.
+move => o [s1 [s2 [-> [/=E2 H]]]]. by rewrite <- E2. move => o H. by exists nil, o. 
 Qed.
 
-Lemma catOPA (P Q R : OPred) : catOP (catOP P Q) R -|- catOP P (catOP Q R).
+Lemma catOPA (P Q R : OPred) : equivOP (catOP (catOP P Q) R) (catOP P (catOP Q R)).
 Proof.
 split. 
-+ move => o [s1 [s2 [-> [[s3 [s4 [-> [H3 H4]]]] H5]]]]. simpl.
++ move => o [s1 [s2 [/=-> [[s3 [s4 [/=-> [H3 H4]]]] H5]]]]. 
   exists s3, (s4++s2). rewrite catA. split => //. split => //. by exists s4, s2. 
-+ move => o [s1 [s2 [-> [H2 [s3 [s4 [-> [H4 H5]]]]]]]]. simpl. 
++ move => o [s1 [s2 [/=-> [H2 [s3 [s4 [/=-> [H4 H5]]]]]]]]. 
   exists (s1++s3), s4. rewrite catA. split => //. split => //. by exists s1, s3. 
 Qed. 
+
+Lemma catOP_trueL P : entailsOP P (catOP trueOP P).
+Proof. move => s H/=. by exists nil, s. Qed.
+
+Lemma catOP_trueR P : entailsOP P (catOP P trueOP). 
+Proof. move => s H/=. exists s, nil. by rewrite cats0. Qed.
+
+Lemma inhabitedOP (O: OPred) : exists s, O s.
+Proof. by destruct O. Qed. 
+
+Lemma catOP_eq_opred (O: OPred) o1 o2 :
+  O o2 ->
+  catOP (eq_opred o1) O (o1++o2).
+Proof. move => H. 
+exists o1, o2. firstorder.  reflexivity. 
+Qed. 
+
+Hint Extern 0 (entailsOP (catOP empOP ?O) ?P) => by apply empOPL.  
+Hint Extern 0 (entailsOP (catOP ?O ?empOP) ?P) => by apply empOPR.  
+
+
+(*
+Local Transparent ILFun_Ops ILPre_Ops.
 
 Lemma land_catOP P Q R : catOP (P//\\Q) R |-- (catOP P R) //\\ (catOP Q R).
 Proof. apply landR. apply catOP_entails_m => //. by apply landL1. 
@@ -94,24 +131,10 @@ Proof. apply landR. apply catOP_entails_m => //. by apply landL1.
                     apply catOP_entails_m => //. by apply landL2. 
 Qed.
 
-Lemma catOP_ltrueL P : P |-- catOP ltrue P.
-Proof. move => s H/=. by exists nil, s. Qed.
-
-Lemma catOP_ltrueR P : P |-- catOP P ltrue.
-Proof. move => s H/=. exists s, nil. by rewrite cats0. Qed.
-
 Lemma catOP_lfalseL P : catOP lfalse P -|- lfalse.
 Proof. split => //. by move => s [s1 [s2 [H1 [H2 H3]]]]/=. Qed. 
 
 Lemma catOP_lfalseR P : catOP P lfalse -|- lfalse.
 Proof. split => //. by move => s [s1 [s2 [H1 [H2 H3]]]]/=. Qed. 
 
-Lemma catOP_eq_opred (O: OPred) o1 o2 :
-  O o2 ->
-  catOP (eq_opred o1) O (o1++o2).
-Proof. move => H. 
-exists o1, o2. firstorder.  reflexivity. 
-Qed. 
-
-Hint Extern 0 (catOP empOP ?O |-- ?P) => by rewrite -> empOPL.  
-Hint Extern 0 (catOP ?O ?empOP |-- ?P) => by rewrite -> empOPR.  
+*)
