src/obs.v
@@ -29,17 +29,17 @@ Qed.
 Local Transparent ILFun_Ops ILPre_Ops.
 
 (* Morphism for obs *)
-Instance obs_entails_m: Proper (lentails ==> lentails) obs.
+Instance obs_entails_m: Proper (entailsOP ==> lentails) obs.
 Proof.
 move => O O' HO k R H1 s H2.  
 destruct (H1 s H2) as [o1 [H3 H5]]. 
 exists o1. by split; [apply: HO |].
 Qed. 
 
-Instance obs_equiv_m: Proper (lequiv ==> lequiv) obs.
-Proof. move => O O' HO. split; [by rewrite HO | by rewrite <-HO]. Qed. 
+Instance obs_equiv_m: Proper (equivOP ==> lequiv) obs.
+Proof. move => O O' [HO HO']. split; by apply obs_entails_m. Qed. 
 
-Lemma safeAsObs : safe -|- obs ltrue. 
+Lemma safeAsObs : safe -|- obs trueOP. 
 Proof. 
 apply spec_equiv => k R. 
 rewrite /safe/obs/mkspec/spec_fun/=.  
@@ -70,6 +70,29 @@ specialize (H _ H1). clear H0 H1.
 destruct H as [o1 [H4 H5]]. 
 exists (o++o1). split. by apply catOP_eq_opred. 
 apply: runsToWith_runsForWithPrefixOf. apply RED. done. 
+Qed. 
+
+Lemma oneStepLaterObs s o s':
+  oneStep s o s' ->
+  forall O,
+  |> obs O @ eq_pred s' |-- obs (catOP (eq_opred o) O) @ eq_pred s.
+Proof. move => RED O k0 R /=H s0 H0.
+have H1 := eq_pred_aux s' H0. 
+rewrite -(eq_pred_aux2 H0). 
+destruct k0. 
+destruct (inhabitedOP O) as [o' Ho']. rewrite /runsForWithPrefixOf/manyStep.
+exists (o++o').
+split.  
+by apply catOP_eq_opred.
+exists s. exists nil. split => //. by exists (o++o'). 
+
+have LT: (k0 < k0.+1)%coq_nat by done. specialize (H _ LT s' H1).
+destruct H as [o' [Ho [s1 [o1 [PRE RUNS]]]]].
+rewrite /runsForWithPrefixOf/manyStep-/manyStep. 
+exists (o++o').
+split. by apply catOP_eq_opred.
+exists s1. eexists _. split; last first. eexists s', o, o1. 
+intuition. by apply cat_preActions. 
 Qed. 
 
 Instance AtEx_obs O: AtEx (obs O).
