src/x86/instrrules/ret.v
@@ -11,6 +11,6 @@ Lemma RET_rule p' (sp:DWORD) (offset:WORD) (p q: DWORD) O :
          obs O @ (EIP ~= p  ** ESP ~= sp  ** sp :-> p')
     ) <@ (p -- q :-> RETOP offset).
 Proof.
-  apply TRIPLE_safe => R. 
+  apply TRIPLE_safeLater => R. 
   do_instrrule_triple.
 Qed.
